towards unified infra

Clap/Lang/FB/FB.lean
@@ -1,4 +1,5 @@
 import Clap.Lang.F.F
+import Clap.eDSLState.Spec
 
 namespace Clap.Edsl.Lang
 
@@ -22,7 +23,7 @@ def toBool (x : FB p) (varStore : ℕ → Option (ZMod p)) : Bool :=
   x.eval varStore == .some 1
 
 def ofBool (p : ℕ) [Fact (p ≥ 2)] (x : Bool) : FB p :=
-  if x then FB.true p else FB.false p
+  if x then FB.true p else FB.false p  
 
 @[simp, grind .] -- TODO(provisional `simp`)
 lemma eval_ofBool_toBool_of_isValid
@@ -62,57 +63,13 @@ lemma equiv (varStore) (b) : FixedExp.eval varStore (ofBool p b) =
 
 end ofBool
 
-abbrev withΓ (p : ℕ) (α ω : Type) := (ℕ → Option (ZMod p)) → α → ω
-
-class IsValid (p : ℕ) (α : Type) where
-  isValid : withΓ p α Prop
-
-def Result (p : ℕ) (α : Type) := α × CircuitResult p
-
-def Result.isPure (result : Result p (ZMod p)) := result.2 = default
-
-/--
-`eval` is allowed to depend on `numAlloc`
--/
-class Eval (p : ℕ) (α : Type) (β : outParam Type) where
-  eval : ℕ → withΓ p α (Result p β)
-
-instance : Eval p (FB p) (ZMod p) := ⟨fun _numAlloc Γ x ↦ ⟨x.eval Γ |>.getD 0, default⟩⟩
-
-class VarStoreSize (p : ℕ) (α : Type) where
-  size : ℕ
-  toLinear : (ℕ → Option (ZMod p)) → α → Vector (ZMod p) size
-
-class Convert (p : ℕ) (representsT idealT : Type) extends IsValid p representsT, VarStoreSize p representsT where
-  toIdeal : (ℕ → Option (ZMod p)) → representsT → Option idealT
-  toRepresents : idealT → representsT
-  someOfIsValid :
-    ∀ (varStore : ℕ → Option (ZMod p)) (x : representsT),
-      isValid varStore x → (toIdeal varStore x).isSome
-  toIdealtoRepresents :
-    ∀ (varStore : ℕ → Option (ZMod p)) (x : idealT),
-      toIdeal varStore (toRepresents x) = .some x
-  toRepresentstoIdeal :
-    ∀ (varStore : ℕ → Option (ZMod p)) (x : representsT),
-      (h : isValid varStore x) →
-        toIdeal varStore (toRepresents ((toIdeal varStore x).get (someOfIsValid varStore x h))) =
-        toIdeal varStore x
-
-def varStoreSize (p : ℕ) (α : Type) [φ : VarStoreSize p α] : ℕ := φ.size
-
-@[grind .]
-lemma someOfIsValid_of_convert {p} {α β : Type} [Convert p α β]
-  {varStore : ℕ → Option (ZMod p)} {x : α} (h : FB.IsValid.isValid varStore x) :
-  (Convert.toIdeal (idealT := β) varStore x).isSome := by
-  aesop (add safe cases Convert)
-
-@[grind .]
-lemma toIdealtoRepresents_of_convert {p} {α β : Type} [Convert p α β]
-  {varStore : ℕ → Option (ZMod p)} {x : β} :
-  Convert.toIdeal (representsT := α) varStore (Convert.toRepresents p x) = .some x := by
-  aesop (add safe cases Convert)
-
 instance : IsValid p (FB p) := ⟨fun Γ a ↦ FB.isValid a Γ⟩
+
+omit [Fact (p ≥ 2)] in
+lemma isValid_iff {varStore} {x} :
+  IsValid.isValid (α := FB p) varStore x ↔
+  x.eval varStore = .some 0 ∨
+  x.eval varStore = .some 1 := by rfl
 
 instance {p} : VarStoreSize p (FB p) where
   size := 1
@@ -125,80 +82,18 @@ instance : Convert p (FB p) Bool where
   toIdealtoRepresents := by simp
   toRepresentstoIdeal := by simp
 
--- class ΓConsistent (α : Type) where
---   Γconsistent : ℕ → Prop
+/-
+TODO Provisional simp
+-/
+attribute [simp, grind =] Convert.toIdealtoRepresents Convert.toRepresentstoIdeal 
 
--- instance : ΓConsistent (FB )
+lemma toIdeal_def {varStore} {x} :
+  Convert.toIdeal (representsT := FB p) (idealT := Bool) varStore x =
+  .some (FB.toBool x varStore) := rfl
 
--- def matchesUnaryBitVecFunctionWithSideEffects
---   {length: ℕ}
---   (p : ℕ)
---   [Fact (p ≥ 2)]
---   (spec_function : (ZMod p) → Vector Bool length)
---   (function : (F p) → Edsl.CircuitStateM p (Vector (FB p) length))
---   (allocates : ℕ)
--- : Prop :=
---   ∀ (a : F p) varStorePre numAllocPre,
---   a.isValid (varStorePre.get?) →
---   let a_eval := (a.eval varStorePre.get?).getD 0
---   let ⟨result, numAllocPost, varStorePost, constraints⟩ := runAndEval (function a) numAllocPre varStorePre
---   result.map (FB.toBool · varStorePost.get?) = spec_function a_eval ∧
---   constraints = True ∧
---   numAllocPost = numAllocPre + allocates ∧
---   ∀ i < numAllocPre, varStorePost.get? i = varStorePre.get? i ∧
---   ∀ (i: Fin length),
---     varStorePost.get? (numAllocPost - i) =
---     .some (((spec_function a_eval).get ⟨length - 1 - i, by {
---       omega
---     }⟩).toNat)
-
-open Convert in
-def matchesUnaryFunction (p : ℕ)
-  {funIn funOut specIn specOut : Type}
-  [Convert p funIn specIn] [Convert p funOut specOut]
-  (spec_function : specIn → specOut)
-  (function : funIn → funOut) : Prop :=
-  ∀ (a : funIn) (varStorePre : ℕ → Option (ZMod p)),
-    (h : IsValid.isValid varStorePre a) →
-      letI aVal : specIn := toIdeal varStorePre a |>.get (someOfIsValid _ _ h)
-      letI leftEval : Option specOut := toIdeal varStorePre (function a)
-      letI wrapped : funOut := toRepresents p (spec_function aVal)
-      leftEval = toIdeal varStorePre wrapped
-
-def assertMatchesLast {k} (varStore : ℕ → Option (ZMod p)) (numAlloc : ℕ) (vec : Vector (ZMod p) k) : Prop :=
-  ∀ i < k,
-    letI varStoreIdx := numAlloc - k + i
-    varStore varStoreIdx = vec[i]?
-
-open Convert VarStoreSize in
-def matchesUnaryMonadFunction (p : ℕ)
-  {funIn funOut specIn specOut : Type}
-  [Convert p funIn specIn] [Convert p funOut specOut]
-  (spec_function : specIn → specOut)
-  (function : funIn → CircuitStateM p funOut)
-  (allocatesN : ℕ)
-  (constraints : Prop) : Prop :=
-  ∀ (a : funIn) (varStorePre : Std.ExtTreeMap ℕ (ZMod p)) (numAllocPre : ℕ),
-    (h : IsValid.isValid varStorePre.get? a) →
-      letI aVal : specIn := toIdeal varStorePre.get? a |>.get (someOfIsValid _ _ h)
-      let ⟨result, circuit⟩ : funOut × CircuitResult p :=
-        CircuitStateM.runAndEval (function a) numAllocPre varStorePre
-      let resultIsValid := IsValid.isValid circuit.varStore.get? result
-      letI resultVal : Option specOut := toIdeal circuit.varStore.get? result
-      letI wrapped : funOut := toRepresents p (spec_function aVal)
-      let resultCorrect := resultVal = toIdeal varStorePre.get? wrapped
-      let constraintsCorrect := circuit.constraints = constraints
-      let allocatesCorrect := circuit.numAlloc = numAllocPre + allocatesN
-      let frameRule := ∀ n < numAllocPre, circuit.varStore[n]? = varStorePre[n]?
-      letI resultSize : ℕ := varStoreSize p funOut
-      letI linearRepr := toLinear circuit.varStore.get? result
-      let resultInVarStore := assertMatchesLast circuit.varStore.get? circuit.numAlloc linearRepr
-      resultIsValid ∧
-      resultCorrect ∧
-      constraintsCorrect ∧
-      allocatesCorrect ∧
-      frameRule ∧
-      resultInVarStore
+lemma toRepresents_def {x} :
+  Convert.toRepresents p (representsT := FB p) (idealT := Bool) x =
+  FB.ofBool p x := rfl
 
 end FB
 
