Clap/Lang/FB/not.lean
@@ -6,16 +6,14 @@ def not {p : ℕ} [Fact (p ≥ 2)] (a : FB p) : FB p := 1 - a
 
 namespace not
 
-def spec (p : ℕ) [Fact (p ≥ 2)] : Prop := matchesUnaryFunction p (!·) FB.not
+def spec (p : ℕ) [Fact (p ≥ 2)] : Prop := matchesUnaryFunction p (!·) (FB.not (p := p))
 
 lemma equiv {p : ℕ} [Fact (p ≥ 2)] :
   spec p
 := by
   intro a varStore h_isValid
-  aesop (add simp [
-    FB.not,left_inv,right_inv,toBool,FB.false,FB.true,isValid,
-    beq_eq_false_iff_ne.mpr, ofBool, FixedExp.eval
-  ])
+  -- NB `Convert.toIdealtoRepresents` in `simp` magics a lot of the reasoning away
+  aesop (add simp [FB.isValid_iff, FB.toIdeal_def, FB.not, toBool])
 
 end not
 
