Clap/eDSLState/Spec.lean
@@ -1,0 +1,93 @@
+import Mathlib.Data.ZMod.Basic
+import Clap.eDSLState.Monad
+
+namespace Clap
+
+abbrev withΓ (p : ℕ) (α ω : Type) := (ℕ → Option (ZMod p)) → α → ω
+
+class IsValid (p : ℕ) (α : Type) where
+  isValid : withΓ p α Prop
+
+class VarStoreSize (p : ℕ) (α : Type) where
+  size : ℕ
+  toLinear : (ℕ → Option (ZMod p)) → α → Vector (ZMod p) size
+
+class Convert (p : ℕ) (representsT idealT : Type) extends IsValid p representsT, VarStoreSize p representsT where
+  toIdeal : (ℕ → Option (ZMod p)) → representsT → Option idealT
+  toRepresents : idealT → representsT
+  someOfIsValid :
+    ∀ (varStore : ℕ → Option (ZMod p)) (x : representsT),
+      isValid varStore x → (toIdeal varStore x).isSome
+  toIdealtoRepresents :
+    ∀ (varStore : ℕ → Option (ZMod p)) (x : idealT),
+      toIdeal varStore (toRepresents x) = .some x
+  toRepresentstoIdeal :
+    ∀ (varStore : ℕ → Option (ZMod p)) (x : representsT),
+      (h : isValid varStore x) →
+        toIdeal varStore (toRepresents ((toIdeal varStore x).get (someOfIsValid varStore x h))) =
+        toIdeal varStore x
+
+def varStoreSize (p : ℕ) (α : Type) [φ : VarStoreSize p α] : ℕ := φ.size
+
+@[grind .]
+lemma someOfIsValid_of_convert {p} {α β : Type} [Convert p α β]
+  {varStore : ℕ → Option (ZMod p)} {x : α} (h : IsValid.isValid varStore x) :
+  (Convert.toIdeal (idealT := β) varStore x).isSome := by
+  aesop (add safe cases Convert)
+
+@[grind .]
+lemma toIdealtoRepresents_of_convert {p} {α β : Type} [Convert p α β]
+  {varStore : ℕ → Option (ZMod p)} {x : β} :
+  Convert.toIdeal (representsT := α) varStore (Convert.toRepresents p x) = .some x := by
+  aesop (add safe cases Convert)
+
+open Convert in
+def matchesUnaryFunction (p : ℕ)
+  {funIn funOut specIn specOut : Type}
+  [Convert p funIn specIn] [Convert p funOut specOut]
+  (spec_function : specIn → specOut)
+  (function : funIn → funOut) : Prop :=
+  ∀ (a : funIn) (varStorePre : ℕ → Option (ZMod p)),
+    (h : IsValid.isValid varStorePre a) →
+      letI aVal : specIn := toIdeal varStorePre a |>.get (someOfIsValid _ _ h)
+      letI leftEval : Option specOut := toIdeal varStorePre (function a)
+      letI wrapped : funOut := toRepresents p (spec_function aVal)
+      leftEval = toIdeal varStorePre wrapped
+
+def assertMatchesLast {k} {p}
+  (varStore : ℕ → Option (ZMod p)) (numAlloc : ℕ) (vec : Vector (ZMod p) k) : Prop :=
+  ∀ i < k,
+    letI varStoreIdx := numAlloc - k + i
+    varStore varStoreIdx = vec[i]?
+
+open Convert VarStoreSize Edsl in
+def matchesUnaryMonadFunction (p : ℕ)
+  {funIn funOut specIn specOut : Type}
+  [Convert p funIn specIn] [Convert p funOut specOut]
+  (spec_function : specIn → specOut)
+  (function : funIn → CircuitStateM p funOut)
+  (allocatesN : ℕ)
+  (constraints : Prop) : Prop :=
+  ∀ (a : funIn) (varStorePre : Std.ExtTreeMap ℕ (ZMod p)) (numAllocPre : ℕ),
+    (h : IsValid.isValid varStorePre.get? a) →
+      letI aVal : specIn := toIdeal varStorePre.get? a |>.get (someOfIsValid _ _ h)
+      let ⟨result, circuit⟩ : funOut × CircuitResult p :=
+        CircuitStateM.runAndEval (function a) numAllocPre varStorePre
+      let resultIsValid := IsValid.isValid circuit.varStore.get? result
+      letI resultVal : Option specOut := toIdeal circuit.varStore.get? result
+      letI wrapped : funOut := toRepresents p (spec_function aVal)
+      let resultCorrect := resultVal = toIdeal varStorePre.get? wrapped
+      let constraintsCorrect := circuit.constraints = constraints
+      let allocatesCorrect := circuit.numAlloc = numAllocPre + allocatesN
+      let frameRule := ∀ n < numAllocPre, circuit.varStore[n]? = varStorePre[n]?
+      letI resultSize : ℕ := varStoreSize p funOut
+      letI linearRepr := toLinear circuit.varStore.get? result
+      let resultInVarStore := assertMatchesLast circuit.varStore.get? circuit.numAlloc linearRepr
+      resultIsValid ∧
+      resultCorrect ∧
+      constraintsCorrect ∧
+      allocatesCorrect ∧
+      frameRule ∧
+      resultInVarStore
+
+end Clap
